scheduler/SchTactics.v
@@ -18,7 +18,7 @@ Section wsim.
   Context (ps pt : bool).
   Context (st_src st_tgt : state).
 
-  Lemma wsim_yield_tgt (src_some : bool) (E : coPset) (q : Qp)
+  Lemma wsim_yield_tgt (tid_res : bool) (E : coPset) (q : Qp)
       (r g : rel)
       (img_s img_t : bool)
       (msk_s msk_t : string → bool)
@@ -27,16 +27,16 @@ Section wsim.
       (k_s : () → itree crisE R_s)
       (k_t : () → itree crisE R_t)
       (my_tid : nat) :
-    (src_some = false ∧
+    (tid_res = false ∧
      sp_s SchHdr.yield = None ∧
      sp_t SchHdr.yield = None ∧
      E = ∅ ∧
      q = 1%Qp (* unused value *)) ∨
-    (src_some = true ∧
+    (tid_res = true ∧
      ∃ sp_user_s,
        sp_incl (SchAS.sp sp_user_s E q) sp_s ∧ img_s = true ∧
        sp_t SchHdr.yield = None) ∨
-    (src_some = true ∧
+    (tid_res = true ∧
     ∃ sp_user_s sp_user_t E_s E_t q_s q_t,
       sp_incl (SchAS.sp sp_user_s E_s q_s) sp_s ∧ img_s = true ∧
       sp_incl (SchAS.sp sp_user_t E_t q_t) sp_t ∧ img_t = true ∧
@@ -44,45 +44,43 @@ Section wsim.
       (q_s ≡ q_t + q)%Qp) →
     msk_s SchHdr.yield →
     msk_t SchHdr.yield →
-    Ist st_src st_tgt ∗ (if src_some then tid_user q my_tid else emp) ∗
-    (∀ st_src st_tgt (NODS: List.NoDup (List.map fst st_src)) (NODT: List.NoDup (List.map fst st_tgt)),
-      Ist st_src st_tgt -∗ (if src_some then tid_user q my_tid else emp) -∗
+    Ist st_src st_tgt ∗ (if tid_res then tid_user q my_tid else emp) ∗
+    (∀ st_src st_tgt,
+      Ist st_src st_tgt -∗ (if tid_res then tid_user q my_tid else emp) -∗
       wsim fl_s fl_t Ist (E, E) r g R_s R_t RR true true
-        (st_src, (SB.sandbox img_s msk_s scp_s (SModTr.trans sp_s Sch.yield)) >>= k_s)
+        (st_src, (SB.sandbox img_s msk_s scp_s (SModTr.trans sp_s 𝒴)) >>= k_s)
         (st_tgt, k_t tt))
     ⊢ wsim fl_s fl_t Ist (E, E) r g R_s R_t RR ps pt
-    (st_src, (SB.sandbox img_s msk_s scp_s (SModTr.trans sp_s Sch.yield)) >>= k_s)
-    (st_tgt, (SB.sandbox img_t msk_t scp_t (SModTr.trans sp_t Sch.yield)) >>= k_t).
-  Proof.
+    (st_src, (SB.sandbox img_s msk_s scp_s (SModTr.trans sp_s 𝒴)) >>= k_s)
+    (st_tgt, (SB.sandbox img_t msk_t scp_t (SModTr.trans sp_t 𝒴)) >>= k_t).
+  Proof using.
     intros Hcase Hmsks Hmskt. iIntros "[IST [TID SIM]]".
     rewrite /Sch.yield; unseal "Sch".
     iStopProof.
     revert st_src. combine_quant st_tgt.
     combine_quant ps. combine_quant pt.
-    eapply wsim_coind.
-    iIntros (g' [pt [ps [st_t st_s]]]). destruct_quant.
-    iIntros "[IST [TID SIM]] %Hg #CIH".
-    unfold_iter_r. steps_r. destruct _q; cycle 1.
-    { unfold_iter_l. steps_l. force_l (Some false). steps_l.
-      steps_r. iApply wsim_nodup. iIntros (? ?).
-      iPoseProof ("SIM" $! _ _ NODS NODT with "IST TID") as "SIM".
+    eapply wsim_coind. intros g' Hg CIH [pt [ps [st_t st_s]]].
+    s; destruct_quant CIH. iIntros "[IST [TID SIM]]".
+    unfold_iterC_r. steps_r. destruct _q; cycle 1.
+    { unfold_iterC_l. steps_l. force_l (Some false). steps_l. steps_r.
+      iPoseProof ("SIM" $! _ _ with "IST TID") as "SIM".
       iPoseProof (wsim_mono_knowledge with "SIM") as "SIM"; cycle 2.
       { iApply "SIM". }
       { iIntros (???????) "$"; done. }
       { iIntros (???????) "P !>". iApply Hg; ss. }
     }
     destruct b; cycle 1.
-    { unfold_iter_l. steps_l. force_l (Some false). steps_l.
-      steps_r. by_coind "CIH". iFrame.
+    { unfold_iterC_l. steps_l. force_l (Some false). steps_l.
+      steps_r. by_coind CIH. iFrame.
     }
-    unfold_iter_l. steps_l. force_l (Some true). steps_l.
+    unfold_iterC_l. steps_l. force_l (Some true). steps_l.
     steps_r.
 
     destruct Hcase as [Hcase|[Hcase|Hcase]]; des; subst.
     { rewrite Hcase0 Hcase1 /=.
       call "IST".
       steps_l. steps_r. hss. steps_l. steps_r.
-      by_coind "CIH". iFrame.
+      by_coind CIH. iFrame.
     }
     { replace (sp_s SchHdr.yield) with (Some (SchAS.yield_spec E q)); cycle 1.
       { erewrite (proj2 Hcase0); et. unfold sp; unseal CRIS; et. }
@@ -91,7 +89,7 @@ Section wsim.
       steps_l.
       call "IST".
       steps_l. iDestruct "ASM" as "[[-> TID] ->]". hss. steps_l. steps_r.
-      by_coind "CIH". iFrame.
+      by_coind CIH. iFrame.
     }
     { replace (sp_s SchHdr.yield) with (Some (SchAS.yield_spec E_s q_s)); cycle 1.
       { erewrite (proj2 Hcase0); et. unfold sp; unseal CRIS; et. }
@@ -110,20 +108,21 @@ Section wsim.
       iPoseProof (tid_user_split with "[TID]") as "[TID0 TID]"; et.
       steps_r. forces_r. iSplitL "TID0"; et.
       steps_r. hss. steps_r.
-      by_coind "CIH". iFrame.
+      by_coind CIH. iFrame.
     }
   (*SLOW*)Qed.
 
   Lemma wsim_yield_src Ep r g img_s (msk_s: _ → bool) sc_s sp_s k_s i_t :
     wsim fl_s fl_t Ist Ep r g R_s R_t RR true pt (st_src, k_s tt) (st_tgt, i_t) ⊢
     wsim fl_s fl_t Ist Ep r g R_s R_t RR true pt
-      (st_src, (SB.sandbox img_s msk_s sc_s (SModTr.trans sp_s Sch.yield)) >>= k_s) (st_tgt, i_t).
+      (st_src, (SB.sandbox img_s msk_s sc_s (SModTr.trans sp_s 𝒴)) >>= k_s) (st_tgt, i_t).
   Proof using.
     iIntros "SIM".
     rewrite /Sch.yield; unseal "Sch".
-    unfold_iter_l; steps_l.
+    unfold_iterC_l; steps_l.
     force_l None; steps_l. iApply "SIM".
   (*SLOW*)Qed.
+
 End wsim.
 
 Ltac sch_yield_l :=
@@ -132,15 +131,140 @@ Ltac sch_yield_l :=
 Ltac sch_resolve :=
   esplits; et; try set_solver.
 
-Ltac sch_yield_rr :=
-  norm_r with do 1 iApply wsim_yield_tgt; [left; sch_resolve|et|et|].
-Ltac sch_yield_ir :=
-  norm_r with do 1 iApply wsim_yield_tgt; [right; left; sch_resolve|et|et|].
-Ltac sch_yield_ii :=
-  norm_r with do 1 iApply wsim_yield_tgt; [right; right; sch_resolve|et|et|].
+Ltac sch_auto :=
+  hrepeat first [progress iFrame | iSplit; iFrame; et; []].
 
 Ltac sch_intros :=
-  try match goal with [H: nat |- _] => clear H end;
-  (do 2 try match goal with [H: List.NoDup (map fst _) |- _] => clear H end);
-  (do 2 try match goal with [H: list (key * Any.t) |- _] => clear H end);
-  iIntros (????); iIntrosFresh "IST"; iIntrosFresh "TID".
+  iIntros (??); iIntrosFresh "IST"; iIntrosFresh "TID";
+  try match goal with [|- context[environments.Esnoc _ ?H (emp%I)]] => iClear H end.
+
+Ltac sch_yield_rr :=
+  norm_r with do 1 iApply wsim_yield_tgt;
+  [left; sch_resolve|et|et|sch_auto; [..|try sch_intros]].
+  
+Ltac sch_yield_ir :=
+  norm_r with do 1 iApply wsim_yield_tgt;
+  [right; left; sch_resolve|et|et|sch_auto; [..|try sch_intros]].
+
+Ltac sch_yield_ii :=
+  norm_r with do 1 iApply wsim_yield_tgt;
+  [right; right; sch_resolve|et|et|sch_auto; [..|try sch_intros]].
+
+Section FancyReal.
+  Context `{!crisG Γ Σ α β τ _S _I, !schG}.
+
+  Context (fl_s fl_t : alist (option string) (Any.t → itree crisE Any.t)).
+  Context (Ist : ist_type Σ).
+  Context (R_s R_t : Type).
+
+  Context (r g : rel).
+  Context (RR : post R_s R_t).
+  Context (ps pt : bool).
+  Context (st_s st_t : state).
+
+  Local Notation sim Ep r g := (wsim fl_s fl_t Ist Ep r g R_s R_t).
+
+  Lemma wsim_real_peek_both
+    X_s X_t (cond_s: X_s → _) (cond_t: X_t → _) k_s k_t
+    img_s img_t (msk_s msk_t: _ → bool) scp_s scp_t
+    :
+    msk_s SchHdr.yield →
+    msk_t SchHdr.yield →
+    Ist st_s st_t ∗
+    (□ ∀ x_s, ∃ x_t, cond_s x_s ==∗ cond_t x_t ∗ (cond_t x_t ==∗ cond_s x_s)) ∗
+    (∀ st_src st_tgt,
+      Ist st_src st_tgt -∗ 
+      sim (∅,∅) r g RR true true (st_src, k_s ()) (st_tgt, k_t ()))
+    ⊢
+    sim (∅,∅) r g RR ps pt
+      (st_s, SB.sandbox img_s msk_s scp_s (SModTr.trans sp_none (real_peek cond_s 𝒴)) >>= k_s)
+      (st_t, SB.sandbox img_t msk_t scp_t (SModTr.trans sp_none (real_peek cond_t 𝒴)) >>= k_t).
+  Proof.
+    i. iIntros "H". iApply wsim_reset. iStopProof.
+    revert st_s. combine_quant st_t.
+    eapply wsim_coind. intros g' Hg CIH [st_t st_s].
+    iIntros "[IST [#COND SIM]] /=". destruct_quant CIH.
+    
+    rewrite /real_peek. unfold_iter_l. steps_l. unfold_iter_r. steps_r.
+    sch_yield_rr. sch_yield_l.
+    steps_r. force_l _q. destruct _q; cycle 1; steps_l; steps_r.
+    { iApply wsim_mono_knowledge; cycle 2.
+      { iApply ("SIM" with "[IST]"); et. }
+      { et. }
+      { i. rewrite Hg. et. }
+    }
+
+    ru_r. iIntros (?) "UPD".
+    ru_l (Own pr)%I. iSplitL "UPD".
+    { iIntros (?) "CS". iDestruct ("COND" $! x) as "[% H]".
+      iMod ("H" with "CS") as "[CT R]".
+      iMod ("UPD" with "CT") as "[PR CT]".
+      iMod ("R" with "CT") as "R". iFrame. et.
+    }
+    iIntros "PR"; force_r; iFrame.
+
+    steps_l; steps_r.
+    by_coind CIH; iFrame; et.
+  Unshelve. all: exact 0.
+  Qed.
+
+  Lemma wsim_real_peek_tgt
+    {X} cond (x: X) E (tid_res : bool) q my_tid
+    k_s k_t img_s img_t (msk_s msk_t: _ → bool) scp_s scp_t sp_s
+    I
+    :
+    (tid_res = false ∧
+     sp_s SchHdr.yield = None ∧
+     E = ∅ ∧
+     q = 1%Qp (* unused value *)) ∨
+    (tid_res = true ∧
+     ∃ sp_user_s,
+       sp_incl (SchAS.sp sp_user_s E q) sp_s ∧ img_s = true) →
+    msk_s SchHdr.yield →
+    msk_t SchHdr.yield →
+    I ∗ Ist st_s st_t ∗ (if tid_res then SchAS.tid_user q my_tid else emp) ∗
+    (□ (∀ st_src st_tgt,
+        I ∗ Ist st_src st_tgt ∗ (if tid_res then SchAS.tid_user q my_tid else emp) ==∗
+        cond x ∗ (cond x ==∗ I ∗ Ist st_src st_tgt ∗ (if tid_res then SchAS.tid_user q my_tid else emp)))) ∗
+    (∀ st_src st_tgt,
+     I ∗ Ist st_src st_tgt ∗ (if tid_res then SchAS.tid_user q my_tid else emp) -∗
+     sim (E,E) r g RR true true
+        (st_src, SB.sandbox img_s msk_s scp_s (SModTr.trans sp_s 𝒴) >>= k_s)
+        (st_tgt, k_t ()))
+    ⊢
+    sim (E,E) r g RR ps pt
+      (st_s, SB.sandbox img_s msk_s scp_s (SModTr.trans sp_s 𝒴) >>= k_s)
+      (st_t, SB.sandbox img_t msk_t scp_t (SModTr.trans sp_none (real_peek cond 𝒴)) >>= k_t).
+  Proof.
+    i. iIntros "H". iApply wsim_reset. iStopProof.
+    revert st_s. combine_quant st_t.
+    eapply wsim_coind. intros g' Hg CIH [st_t st_s].
+    iIntros "[I [IST [TID [#COND SIM]]]] /=". destruct_quant CIH.
+    
+    rewrite /real_peek. unfold_iter_r. steps_r.
+    iApply wsim_yield_tgt; [|et|et|try (sch_auto; sch_intros)].
+    { des; subst; [left|right;left]; et. }
+    steps_r. destruct _q; cycle 1; steps_r.
+    { iApply wsim_mono_knowledge; cycle 2.
+      { iApply ("SIM" with "[I IST TID]"); et; iFrame. }
+      { et. }
+      { i. rewrite Hg. et. }
+    }
+
+    ru_r. iIntros (?) "UPD".
+    iMod ("COND" with "[I IST TID]") as "[C R]"; iFrame.
+    iMod ("UPD" with "C") as "[PR C]".
+    iMod ("R" with "C") as "[I [IST TID]]".
+    force_r; iFrame. steps_r.
+    by_coind CIH. iFrame. et.
+  Qed.
+
+End FancyReal.
+
+Ltac fancy_peek_rr :=
+  norm_r with do 1 iApply wsim_real_peek_tgt;
+  [left; sch_resolve|et|et|sch_auto; [..|try sch_intros]].
+
+Ltac fancy_peek_ir :=
+  norm_r with do 1 iApply wsim_real_peek_tgt;
+  [right; sch_resolve|et|et|sch_auto; [..|try sch_intros]].
